%%%
\chapter{Learning Lens}


The content of this chapter comes fron Simon Peyton Jones's \href{https://skillsmatter.com/skillscasts/4251-lenses-compositional-data-access-and-manipulation}{Lenses: Compositional data access and mainpulation} talk.

\section{Native Approach}

\begin{minted}{haskell}
data Person = Person { name    :: String,
                     , address :: Address
                     , salary  :: Int }

data Address = Address { road :: String
                       , city :: String
                       , zip  :: String }
\end{minted}

The goals for lens

* To access and update a given field
* Compose Lense

\begin{minted}{haskell}
data LensR s a = LensR { viewR :: s -> a
                       , setR  :: a -> s -> s }
\end{minted}

\begin{minted}{haskell}
data Prisms s a = Prisms { match :: s -> Either s a
                         , build :: a -> s}
\end{minted}

Type `s` represent the overall record we try to access or update, Type `a` represent the field we are try to acccess or update.

How to compose `LensR`

\begin{minted}{haskell}
composeL :: LensR s1 s2 -> LensR s2 a -> LensR s1 a
composeL (L v1 s1) (L v2 s2)
    = L (\ s -> v2 (v1 s))
        (\ a s -> s1 (s2 a (v1 s)) s)
\end{minted}

The two big problems with this approach is to inefficent, and inflexiable.

\subsection{A step further on this Native Approach}

\begin{minted}{haskell}
data LensR s a
    = L { viewR :: s -> a
        , setR  :: a -> s -> a
        , mod   :: (a -> a) -> s -> s
        , modM  :: (a -> Maybe a) -> s -> Maybe s
        , modIO :: (a -> IO a) -> s -> IO s }
\end{minted}

The last two (or three if you know your functor well) share lots of commonality.

If we can abstract the common pattern

\begin{minted}{haskell}
data LensR s a
    = L { viewR :: s -> a
        , setR  :: a -> s -> a
        , mod   :: (a -> a) -> s -> s
        , modF  :: Functor f => (a -> f a) -> s -> f s }
\end{minted}



\begin{minted}{haskell}
type Lens' s a = forall f. Functor f => (a -> f a) -> s -> f s
\end{minted}

You may think `Lens'` looks nothing like `LensR`, but they are actually isomorphic.



Side Bar :: Isomorphic

If `A` and `B` are isomorphic, it means we are getting `B` to `A` without lost any information, and vice verse.

Before proving `Lens'` and `LensR` is isomorphic, allow me introduce two oddly looking functors `Const` and `Identity`.


Break Down::
\begin{minted}{haskell}
view :: Lens' s a -> s -> a => ((a -> f a) -> s -> f s) -> s -> a
view ln s = getConst (ln const s)
\end{minted}

\begin{minted}{haskell}
let fred = P {_name = "Fred", _salary = 100}
name :: Lens' Person String
name fn (P n s) -> (\ n' -> P n' s) <$> fn n
\end{minted}

\begin{minted}{haskell}
view name fred
= (getConst . name . const) fred
= getConst ((\n' -> P n' s) <$> Const "Fred")
= getConst . Const "Fred"
= "Fred"
\end{minted}

\begin{minted}{haskell}
set name "John" fred
= getID $ name (Id . Const  "John") fred
= getID $ (\ n' -> P n' 100) <$> ((ID. Const  "John" ) fred)
= getID $ (\ n' -> P n' 100) <$> Id "John"
= getID $ ID (P "John" 100 )
= P "John" 100
\end{minted}


Compose Lens'

Function application

\url{https://www.youtube.com/watch?v=sfWzUMViP0M&t=441s}

\url{https://www.google.com/url?sa=t&rct=j&q=&esrc=s&source=web&cd=1&ved=2ahUKEwiS6dD65PfdAhVSJjQIHRzzC9IQFjAAegQIBBAC&url=http%3A%2F%2Fwww.cs.ox.ac.uk%2Fpeople%2Fjeremy.gibbons%2Fpublications%2Fpoptics.pdf&usg=AOvVaw3KgxUg3x37WIToXgmRu79C}

The problem: heterogeneous composite data

Worse: consider access to the A in a composiation data structure
Maybe (A x B) built using both sums and products.

Sum part comes with Maybe `data Maybe a = Just a | Nothing`


\begin{minted}{haskell}
*Main Lib> import Control.Lens
*Main Lib Control.Lens> ("hello","world") ^. _2
"world"
*Main Lib Control.Lens>
\end{minted}

\section{What is a Lens ?}
Lenses address some part of a “structure” that always exists, either look that part, or set that part.
“structure” can be a computation result, for example, the hour in time. Functional setter and getter.
  Data.Lens


\begin{minted}{haskell}
data Lens s a = Lens { set  :: s -> a -> a
                     , view :: s -> a
                     }
view :: Lens s a -> s -> a
set  :: Lens s a -> s -> a -> s
\end{minted}

view looks up an attribute a from s
view is the getter, and set is the setter.
Laws
1. set l (view l s) s = s
2. view l (set l s a) = a
3. set l (set l s a) b = set l s b
Law 1 indicates lens has no other effects
since set and view in Lens both start with s ->, so we can fuse the two functions into a single function
`s -> (a -> s, a)`.

So we could define Lens as
\begin{minted}{haskell}
data Lens s a = Lens (s -> (a -> s), a)
data Store s a = Store (s -> a) s
data Lens s a = Lens (s -> Store a s)
\end{minted}

Side bar Store Comonad
url{https://stackoverflow.com/questions/8428554/what-is-the-comonad-typeclass-in-haskell}
hurl{ttps://stackoverflow.com/questions/8766246/what-is-the-store-comonad}

Lens can form a category

 Semantic Editor Combinator

The Power is in the dot
\begin{minted}{haskell}
(.)         :: (b -> c) -> (a -> c) -> (a -> c)
(.).(.)     :: (b -> c) -> (a1 -> a2 -> b) -> a1 -> a2 -> c
(.).(.).(.) :: (b -> c) -> (a1 -> a2 -> a3 -> b) -> a1 -> a2 -> a3 -> c
\end{minted}

\href{https://www.reddit.com/r/haskellquestions/comments/ayi445/help_me_understand_the_function_and_its_type}{Detail Explantation}

\begin{minted}{haskell}
(.) :: (b -> c) -> (a -> b) -> a -> c
f . g = \ t -> f (g t)
\end{minted}


\begin{align*}
& ((.).(.)) (+1) (+) 10 10 = 21 \\
&  ((.).(.)) (+1) (+) 10 10 \\
& =  (.)((.) (+1)) (+) 10 10 \\
& =  ((.) (+1)) (+ 10) 10   \\
& = ((+1). (+10)) 10 \\
& = (+1) ((+10) 10) \\
& = (+1) (10 + 10) \\
& = 21
\end{align*}

\begin{minted}{haskell}
(.).(.) :: (b -> c) -> (a -> b) -> a -> c
dotF . dotG :: (b -> c) -> (a -> c) -> a -> c
dotF :: b -> c
dotG :: a -> b
\end{minted}

since \textbf{dotF} is just an alias to  \textbf{(.)}
\begin{equation}
dotF :: (u -> v) -> (s -> u) -> s -> v
(u -> v) -> (s -> u) -> s -> v === b -> c
\end{equation}
therefore

\begin{equation}
b === (u -> v) \\
c === (s -> u) -> s -> v
\end{equation}

`dotG` is also an alias to `(.)`

\begin{equation}
dotG :: (y -> z) -> (x -> y) -> x -> z
(y -> z) -> (x -> y) -> x -> z === a -> b
\end{equation}
therefore

\begin{equation}
a === (y -> z)
b === (x -> y) -> x -> z
\end{equation}

since \textbf{b} appears on both side

\begin{equation}
a === y -> z
b === (u -> v)
b === (x -> y) -> x -> z
c === (s -> u) -> s -> v
\end{equation}

we can deduct

\begin{align*}
u &=== x -> y  \\
v &=== x -> z
\end{align*}

therefore \begin{equation}c === (s -> x -> y) -> s -> x -> z\end{equation}

\begin{align*}
(.).(.) & === a -> c \\
(.).(.) & === (y -> z) -> (s -> x -> y) -> s -> x - z
\end{align*}


we can generalize this to any functor

\begin{minted}{haskell}
fmap                :: Functor f  => (a -> b) -> f a -> f b
fmap . fmap         :: ( Functor f, Functor g)   => (a -> b) -> f (g a) -> f (g b)
fmap . fmap . fmap  :: (Functor f, Functor g, Functor h) => (a -> b) -> f (g (h a)) -> f (g (h b))
\end{minted}

it means we compose a function under arbitrary level deep nested context
Semantic Editor Combinator

`type SEC s t a b = (a -> b) -> s -> t`
it like a functor (a -> b) -> f a -> f b
`fmap` is Semantic Editor Combinator
`fmap . fmap` is also a SEC

so we use `s` to generalize `f a`,  `f (g a)`, `f (g (h a))` and `t` to generalize `f b`,  `f (g b)`, `f (g (h b))`.
It may seems counterintuitive at first, we lost the relation between a and s, b and t.
Functor is a semantic Editor Combinator
`fmap :: Functor f => SEC (f a) (f b) a b`

first is a also SEC ?
\begin{minted}{haskell}
first :: SEC (a, c) (b,c) a b
first f (a, b) = (f a, b)
\end{minted}
Setters
We can compose Traversable the way as we can compose `(.)` and `fmap`

\begin{minted}{haskell}
traverse                       :: (Traversable f, Applicative m) => (a -> m b) -> f a -> m (f b)
traverse . traverse            :: (Traversable f, Traversable g, Applicative m) => (a -> m b) -> f (g a) -> m (f (g b))
traverse . traverse . traverse :: (Traversable f, Traversable g, Traversable h, Applicative m) => (a -> m b) -> f (g (h a)) -> m (f (g (h b)))
\end{minted}

traverse is a generalized version of mapM, and work with any kind of Foldable not just List.

\begin{minted}{haskell}
class (Functor f, Foldable f) => Traversable f where
   traverse :: Applicative m => (a -> m b) -> f a -> m (f b)
\end{minted}

\begin{minted}{haskell}
fmapDefault :: forall t a b. Traverable t => (a -> b) -> t a -> t b
fmapDefault f = runIndentity . traverse (Identity . f)
\end{minted}

build `fmap` out from traverse
we can change `fmapDefault`

\begin{minted}{haskell}
over l f = runIdentity . l (Identity . f)
over traverse f = runIdentity . traverse (Identity . f)
                = fmapDefault f
                = fmap f
\end{minted}

type of `over :: ((a -> Identity b) -> s -> Identity t) -> (a -> b) -> s -> t`
type Setter s t a b = (a -> Identity b) -> s -> Identity t
so we could rewrite `over` as
over :: Setter s t a b -> (a -> b) -> s -> t
let’s apply setter

\begin{minted}{haskell}
mapped :: Functor f => Setter (f a) (f b) a b
mapped f = Identity . fmap (runIdentity . f)
over mapped f = runIdentity . mapped (Identity . f)
              = runIdentity . Identity . fmap (runIdentity . Identity . f)
              - fmap f
\end{minted}

Examples

\begin{minted}{haskell}
over mapped (+1) [1,2,3]  ===> [2,3,4]
over (mapped . mapped) (+1) [[1,2], [3]] ===> [[2,3], [4]]
chars :: (Char -> Identity Char) -> Text -> Identity Text
chars f = fmap pack . mapped f . unpack
\end{minted}

Laws for setters
Functor Laws:
1. `fmap` id = id
2. fmap f . fmap g = fmap (f . g)

Setter Laws for a legal Setter l.
1. over l id = id
2. over l f . over l g = over l (f . g)


Practices
Simplest lens
\verb|(1,2,3) ^. _2   ===> 2|
\verb|view _2 (1, 2, 3)|


 References
\href{https://skillsmatter.com/skillscasts/4251-lenses-compositional-data-access-and-manipulation}{SPJ Lenses: compositional data access and manipulation}
\href{https://www.youtube.com/watch?v=cefnmjtAolY}{Edward Kmett's NYC Haskell Meetup talk}
\href(http://comonad.com/haskell/Lenses-Folds-and-Traversals-NYC.pdf){Edward Kmett's NYC Haskell Meetup talk slide}
\url{http://hackage.haskell.org/package/lens-tutorial-1.0.3/docs/Control-Lens-Tutorial.html}
\url{https://www.youtube.com/watch?v=H01dw-BMmlE}
\url{https://www.youtube.com/watch?v=QZy4Yml3LTY}
\url{https://www.youtube.com/watch?v=T88TDS7L5DY}
\url{http://lens.github.io/tutorial.html}
\url{https://www.reddit.com/r/haskell/comments/9ded97/is_learning_how_to_use_the_lens_library_worth_it/e5hf9ai/}
\url{https://blog.jle.im/entry/lenses-products-prisms-sums.html}
